%' Matrix multiplication
%' 
%' @src: The 1st equation in 'Demystifying Item Response Theory (3/4)' 
%' @url: https://yongfu.name/2023/03/29/irt3/#reconstructing-dropped-estimates
\documentclass[12pt,preview,border=0]{standalone}
\usepackage[paperheight=10cm,paperwidth=14cm]{geometry}
\usepackage{amsmath}

\begin{document}

$$
\begin{bmatrix}
    1 & 0 \\
    0 & 1 \\
    -1 & -1
    \end{bmatrix} 
    \begin{bmatrix}
    E_1 \\
    E_2
    \end{bmatrix} = 
    \begin{bmatrix}
    E_1 \\
    E_2 \\
    -E_1 - E_2
\end{bmatrix}
$$

\end{document}
